Split Schema WF into theory and definitions

src/SchemaWellFormedness.v
@@ -16,11 +16,13 @@ Require Import SchemaAux.
 Section WellFormedness.
 
   Variables (Name Vals : ordType).
-  Implicit Type sch : @schema Name.
 
+  Section Defs.
+    
+    Variable (s : @schema Name).
 
-  
-   (** Subtype relation
+    
+    (** Subtype relation
 
    
                  ----------------------- (ST_Refl)
@@ -42,61 +44,38 @@ Section WellFormedness.
         1. Transitivity : There is no need to specify this because only objects can 
         be subtype of an interface and not between objects. Interfaces cannot be
         subtype of another interface.
-   **)
-  Inductive Subtype sch : type -> type -> Prop :=
-  | ST_Refl : forall ty, Subtype sch ty ty
-                            
-  | ST_Interface : forall n n',
-      declares_implementation sch n n' ->
-      Subtype sch (NT n) (NT n')
-              
-  | ST_Union : forall n n',
-      (n \in (union_members sch n')) ->
-      Subtype sch (NT n) (NT n')
-                    
-  | ST_ListType : forall ty ty',
-      Subtype sch ty ty' ->
-      Subtype sch (ListType ty) (ListType ty'). 
+     **)
+    Inductive Subtype : type -> type -> Prop :=
+    | ST_Refl : forall ty, Subtype ty ty
+                              
+    | ST_Interface : forall n n',
+        declares_implementation s n n' ->
+        Subtype (NT n) (NT n')
+                
+    | ST_Union : forall n n',
+        (n \in (union_members s n')) ->
+        Subtype (NT n) (NT n')
+                
+    | ST_ListType : forall ty ty',
+        Subtype ty ty' ->
+        Subtype (ListType ty) (ListType ty'). 
 
-  Equations is_subtype sch (ty ty' : @type Name) : bool :=
-    {
-      is_subtype sch (ListType lty) (ListType lty') := is_subtype sch lty lty';
+    Equations is_subtype (ty ty' : @type Name) : bool :=
+      {
+        is_subtype (ListType lty) (ListType lty') := is_subtype lty lty';
 
-      is_subtype sch (NT name) (NT name') :=
-        [|| (name == name'),
-         declares_implementation sch name name' | 
-         (name \in (union_members sch name'))];
-      
-      is_subtype _ _ _ := false
-    }.
+        is_subtype (NT name) (NT name') :=
+          [|| (name == name'),
+           declares_implementation s name name' | 
+           (name \in (union_members s name'))];
+        
+        is_subtype _ _ := false
+      }.
 
-   (* Lemma subtypeP sch ty ty': reflect (Subtype sch ty ty') (is_subtype sch ty ty'). *)
-   (* Proof. *)
-   (*  apply: (iffP idP). *)
-   (*  elim: ty ty' => n. *)
-   (*    - case=>  //. *)
-   (*      * by move=> n' /= /or3P [/eqP -> | Hi | Hu]; [apply ST_Refl | apply ST_Interface | apply ST_Union]. *)
-   (*      by move=> IH; case=> // => t' /= /IH; apply ST_ListType. *)
-   (*  elim=> //=. *)
-   (*    - elim=> //=. *)
-   (*      * by move=> *; apply/or3P; constructor 1. *)
-   (*    - by move=> * /=; apply/or3P; constructor 2. *)
-   (*    by move=> * /=; apply/or3P; constructor 3. *)
-   (* Qed. *)
-
-
-   (* Lemma is_subtype_is_same_or_in_possible_types sch (ty ty' : type) :
-     reflect (ty = ty' \/ ty.(tname) \in get_possible_types sch ty')
-             (is_subtype sch  ty ty').
-   Proof.
-     apply: (iffP idP).
-     - move/subtypeP; case => //.
-       * by intros; left.
-       * move=> n n' Hdecl. *)
- 
-     
-         
-  (** The two following definitions describe whether a given type is a valid type
+    
+    
+    
+    (** The two following definitions describe whether a given type is a valid type
       for a field argument (IsValidArgumentType) and if it is a valid type for a field itself 
       (IsValidFieldType).
 
@@ -104,80 +83,50 @@ Section WellFormedness.
 
       https://facebook.github.io/graphql/June2018/#sec-Input-and-Output-Types **)
 
-  Inductive valid_argument_type sch : type -> Prop :=
-  | VScalar_Arg : forall ty,
-      is_scalar_type sch ty ->
-      valid_argument_type sch (NT ty)
-  | VEnum_Arg : forall ty,
-      is_enum_type sch ty ->
-      valid_argument_type sch (NT ty)
-  | VList_Arg : forall ty,
-      valid_argument_type sch ty ->
-      valid_argument_type sch (ListType ty).
-  
-  Fixpoint is_valid_argument_type sch (ty : type) : bool :=
-    match ty with
-    | NT name => is_scalar_type sch ty || is_enum_type sch ty
-    | ListType ty' => is_valid_argument_type sch ty'
-    end.
+    Inductive valid_argument_type  : type -> Prop :=
+    | VScalar_Arg : forall ty,
+        is_scalar_type s ty ->
+        valid_argument_type (NT ty)
+    | VEnum_Arg : forall ty,
+        is_enum_type s ty ->
+        valid_argument_type (NT ty)
+    | VList_Arg : forall ty,
+        valid_argument_type ty ->
+        valid_argument_type (ListType ty).
+    
+    Fixpoint is_valid_argument_type  (ty : type) : bool :=
+      match ty with
+      | NT name => is_scalar_type s ty || is_enum_type s ty
+      | ListType ty' => is_valid_argument_type  ty'
+      end.
 
 
-  Lemma valid_argument_typeP sch : forall ty, reflect (valid_argument_type sch ty) (is_valid_argument_type sch ty).
-  Proof.
-    move=> ty; apply: (iffP idP).
-    elim: ty.
-      - by move=> n /orP [Hs | He]; [apply (VScalar_Arg Hs) | apply (VEnum_Arg He)].
-      by move=> t IH /= /IH; apply VList_Arg.
-    elim=> //.
-       - by move=> n H; apply/orP; left.
-       by move=> n H; apply/orP; right.
-  Qed.
-  
-  (* Because we are not considering InputObjects, a field may have any type, 
+    
+    (* Because we are not considering InputObjects, a field may have any type, 
      as long as it is declared in the Schema. *)
-  Inductive valid_field_type sch : type -> Prop :=
-  | VBase_Type : forall n,
-      is_declared sch n ->
-      valid_field_type sch (NT n)      
-  | VList_Type : forall ty,
-      valid_field_type sch ty ->
-      valid_field_type sch (ListType ty).
-  
-  Fixpoint is_valid_field_type sch (ty : type) : bool :=
-    match ty with
-    | NT n => is_declared sch n
-    | ListType ty' => is_valid_field_type sch ty'
-    end.
-  
+    Inductive valid_field_type  : type -> Prop :=
+    | VBase_Type : forall n,
+        is_declared s n ->
+        valid_field_type (NT n)      
+    | VList_Type : forall ty,
+        valid_field_type ty ->
+        valid_field_type (ListType ty).
+    
+    Fixpoint is_valid_field_type (ty : type) : bool :=
+      match ty with
+      | NT n => is_declared s n
+      | ListType ty' => is_valid_field_type  ty'
+      end.
+    
 
-  Lemma valid_field_typeP sch : forall ty, reflect (valid_field_type sch ty) (is_valid_field_type sch ty).
-  Proof.
-    move=> ty; apply: (iffP idP); last by elim.
-    elim: ty.
-      by move=> n /=; apply VBase_Type.
-      by move=> t H /= /H; apply VList_Type.
-  Qed.
-
-    Lemma obj_subtypeE sch (ty ty' : type) :
-     is_object_type sch ty ->
-     is_subtype sch ty ty' ->
-     [\/ ty' = ty,
-      is_interface_type sch ty' |
-      is_union_type sch ty'].
-    Proof.
-      funelim (is_subtype sch ty ty') => //= Hobj.
-      - case/or3P => [/eqP -> | |]; first by constructor 1. 
-        * (* need conformance *)
-    Abort.
-  
-  (** 
+    (** 
       It checks whether an argument is well-formed by checking that
       its type is a valid type for an argument **)
-  Definition is_field_argument_wf sch (arg : FieldArgumentDefinition) : bool :=
-    is_valid_argument_type sch arg.(argtype).
+    Definition is_field_argument_wf (arg : FieldArgumentDefinition) : bool :=
+      is_valid_argument_type arg.(argtype).
 
-  
-  (**
+    
+    (**
      It states whether a field is well-formed.
 
                  ty isValidFieldType
@@ -185,32 +134,32 @@ Section WellFormedness.
            ∀ arg ∈ args, arg isWellFormed
            ------------------------------
            (fname (args) : ty) isAWellFormedField
-   **)
-  Definition is_field_wf sch (fld : FieldDefinition) : bool :=
-    is_valid_field_type sch fld.(return_type) &&
-     (* uniq [seq arg.(argname) | arg <- fld.(fargs)] &  // Not specified... But should be? *)
-     all (is_field_argument_wf sch) fld.(fargs).
+     **)
+    Definition is_field_wf (fld : FieldDefinition) : bool :=
+      is_valid_field_type fld.(return_type) &&
+                                            (* uniq [seq arg.(argname) | arg <- fld.(fargs)] &  // Not specified... But should be? *)
+                                            all (is_field_argument_wf) fld.(fargs).
 
 
 
-  (** This checks whether an object field is valid w/r to another from an implemented interface.
+    (** This checks whether an object field is valid w/r to another from an implemented interface.
       It checks the following:
       1. Both fields have the same name.
       2. The arguments of the interface field must be a subset of the object's arguments.
       3. The object's field return type must be a subtype of the interface's field.
 
       This is not checking that any additional argument in the object must be a "non-required" field.
-   **)
-  Definition is_field_ok sch (fld fld' : FieldDefinition) : bool :=
-    [&& (fld.(fname) == fld'.(fname)),
-     fsubset fld'.(fargs) fld.(fargs) &
-     is_subtype sch fld.(return_type) fld'.(return_type)].
+     **)
+    Definition is_field_ok (fld fld' : FieldDefinition) : bool :=
+      [&& (fld.(fname) == fld'.(fname)),
+       fsubset fld'.(fargs) fld.(fargs) &
+       is_subtype fld.(return_type) fld'.(return_type)].
     
 
 
 
-  
-  (**
+    
+    (**
      This checks whether an object type implements correctly an interface, 
      by properly defining every field defined in the interface.
 
@@ -221,40 +170,16 @@ Section WellFormedness.
             ------------------------------------------------
                         O implementsOK I
 
-   **)
- (* Inductive implementsOK schema : type -> type -> Prop :=
-  | ImplementsAll : forall name intfs fields iname ifields,
-      lookupName schema name = Some (ObjectTypeDefinition name intfs fields) ->
-      In (NamedType iname) intfs ->
-      lookupName schema iname = Some (InterfaceTypeDefinition iname ifields) ->
-      (forall ifld, In ifld ifields ->
-               exists ofld, In ofld fields ->
-                       fieldOk schema ofld ifld)  ->
-      implementsOK schema (NamedType name) (NamedType iname).
+     **)
+    
+    Definition implements_interface_correctly (ty ty' : NamedType) : bool :=
+      let ifields := fields s ty' in
+      let ofields := fields s ty in
+      all (fun f' => has (fun f => is_field_ok f f') ofields) ifields.
+    
 
-*)
-  Definition implements_interface_correctly sch (ty ty' : NamedType) : bool :=
-    let ifields := fields sch ty' in
-    let ofields := fields sch ty in
-    all (fun f' => has (fun f => is_field_ok sch f f') ofields) ifields.
-     
-
-  Lemma implements_interface_correctlyP sch (ity ty : NamedType) :
-    reflect (forall fi, fi \in fields sch ity ->
-                          exists f, f \in fields sch ty /\ is_field_ok sch f fi)
-            (implements_interface_correctly sch ty ity).
-  Proof.
-    apply: (iffP idP).
-    - rewrite /implements_interface_correctly => /allP H.
-      by move=> fi /H /hasP [f Hin Hok]; exists f.
-    - move=> H.
-      rewrite /implements_interface_correctly.
-      apply/allP => fi Hin.
-      apply/hasP.
-      by move: (H fi Hin) => [f [Hin' Hok]]; exists f.
-  Qed.
-  
-  (**
+    
+    (**
 
                        Schema(S) = scalar S 
                        -----------------------
@@ -294,374 +219,52 @@ Section WellFormedness.
                 -----------------------------------------
                           enum E { Evs } 
 
-   **)
-  
+     **)
+    
 
-  Fixpoint is_type_def_wf sch (tdef : TypeDefinition) : bool :=
-    match tdef with
-    | ScalarTypeDefinition _ => true
-                                 
-    | ObjectTypeDefinition name interfaces fields =>
-      [&& (fields != [::]),
-       uniq [seq fld.(fname) | fld <- fields],
-       all (is_field_wf sch) fields,
-       all (is_interface_type sch) interfaces &
-       all (implements_interface_correctly sch name) interfaces]
+    Fixpoint is_type_def_wf (tdef : TypeDefinition) : bool :=
+      match tdef with
+      | ScalarTypeDefinition _ => true
+                                   
+      | ObjectTypeDefinition name interfaces fields =>
+        [&& (fields != [::]),
+         uniq [seq fld.(fname) | fld <- fields],
+         all (is_field_wf) fields,
+         all (is_interface_type s) interfaces &
+         all (implements_interface_correctly name) interfaces]
 
-    | InterfaceTypeDefinition _ fields =>
-      [&& (fields != [::]),
-       uniq [seq fld.(fname) | fld <- fields] &
-       all (is_field_wf sch) fields]
+      | InterfaceTypeDefinition _ fields =>
+        [&& (fields != [::]),
+         uniq [seq fld.(fname) | fld <- fields] &
+         all (is_field_wf) fields]
 
-    | UnionTypeDefinition name members =>
-      (members != fset0) && all (is_object_type sch) members
+      | UnionTypeDefinition name members =>
+        (members != fset0) && all (is_object_type s) members
 
-    | EnumTypeDefinition _ enumValues => enumValues != fset0
-        
-    end.
+      | EnumTypeDefinition _ enumValues => enumValues != fset0
+                                                     
+      end.
 
-
-  Lemma is_type_def_wf_objE sch name interfaces fields :
-    is_type_def_wf sch (ObjectTypeDefinition name interfaces fields) =
-    [&& (fields != [::]),
-       uniq [seq fld.(fname) | fld <- fields],
-       all (is_field_wf sch) fields,
-       all (is_interface_type sch) interfaces &
-       all (implements_interface_correctly sch name) interfaces].
-  Proof.
-      by case: sch. Qed.
-
-  Lemma is_type_def_wf_unionE sch name mbs :
-    is_type_def_wf sch (UnionTypeDefinition name mbs) = (mbs != fset0) && all (is_object_type sch) mbs.
-  Proof. by case: sch. Qed.
 
     
+    
+    Definition is_schema_wf : bool :=
+      [&& s.(query_type) \in s.(schema_names),
+                             is_object_type s s.(query_type),
+                             all (fun p => has_name p.1 p.2) s.(type_definitions) &
+                             all (fun p => is_type_def_wf p.2) s.(type_definitions)].
+
+  End Defs.
   
-  Definition is_schema_wf sch : bool :=
-    [&& (sch.(query_type) \in schema_names sch),
-     is_object_type sch sch.(query_type),
-     all (fun p => has_name p.1 p.2) sch.(type_definitions) &
-     all (fun p => is_type_def_wf sch p.2) sch.(type_definitions)].
-      
   
   Structure wfSchema := WFSchema {
-                           sch;
+                           sch : @schema Name;
                            hasType :  Name -> Vals -> bool;
                            _ : is_schema_wf sch;
-                      }.
+                         }.
 
   
   Coercion sch : wfSchema >-> Schema.schema.
-
-
-
-  Ltac wfschema := case: schema => sch Hhty; rewrite /is_schema_wf => /= /and4P [Hqin Hqobj Hhn /allP Hok].
-
-  Lemma query_has_object_type (schema : wfSchema) :
-    is_object_type schema schema.(query_type).
-  Proof.
-    by  wfschema.
-  Qed.
-
-
-  Lemma tdefs_N_nil (schema : wfSchema) :
-    schema.(type_definitions) != emptym.
-  Proof.
-    wfschema.
-    rewrite /schema_names in_fset in Hqin.
-    move/mapP: Hqin => [x /codommP [t Hs] Hqin].
-    case: (type_definitions sch) Hs.
-    by case.
-  Qed.
-
-  Lemma lookup_type_name_wf (schema : wfSchema) ty tdef :
-    lookup_type schema ty = Some tdef ->
-    ty = tdef.(tdname).
-  Proof.
-    wfschema.
-    rewrite /lookup_type.
-    move/getmP=> Hin.
-    move/allP: Hhn.
-    by move/(_ (ty, tdef) Hin) => /has_nameP /=.
-  Qed.
-
-  
-
-
-  Lemma lookup_in_schema_wfP (schema : wfSchema) ty tdef :
-    reflect (lookup_type schema ty = Some tdef /\ ty = tdef.(tdname))
-            ((ty, tdef) \in schema.(type_definitions)).
-  Proof.
-    wfschema.
-    apply: (iffP idP).
-    - move=> Hin.
-      move/allP: Hhn.
-      move/(_ (ty, tdef) Hin) => /has_nameP /= Heq.
-      rewrite Heq in Hin *.
-        by move/lookup_in_schemaP: Hin; split.
-    - move=> [Hlook Heq].
-      by apply/lookup_in_schemaP.
-  Qed.
-
- 
-  Lemma is_scalar_type_wfE (schema : wfSchema) ty :
-    reflect (lookup_type schema ty = Some (ScalarTypeDefinition ty))
-            (is_scalar_type schema ty).
-  Proof.
-    apply: (iffP idP).
-    - rewrite /is_scalar_type.
-      case Hlook: lookup_type => [tdef|] //.
-      move/lookup_type_name_wf: Hlook => ->.
-        by case: tdef.
-    - move=> Hlook.
-      by rewrite /is_scalar_type Hlook.
-  Qed.
-
-  Lemma is_object_type_wfP (schema : wfSchema) ty :
-    reflect (exists intfs flds, lookup_type schema ty = Some (ObjectTypeDefinition ty intfs flds))
-            (is_object_type schema ty).
-  Proof.
-    apply: (iffP idP)=> //.
-    - funelim (is_object_type schema ty) => // _.
-      by exists f, l; rewrite Heq; move/lookup_type_name_wf: Heq => ->.
-    - move=> [intfs [flds Hlook]].
-        by rewrite is_object_type_equation_1 Hlook.
-  Qed.
-
-  Lemma is_interface_type_wfP (schema : wfSchema) ty :
-    reflect (exists flds, lookup_type schema ty = Some (InterfaceTypeDefinition ty flds))
-            (is_interface_type schema ty).
-  Proof.
-    apply: (iffP idP).
-    - funelim (is_interface_type schema ty) => // _.
-        by exists l0; rewrite Heq; move/lookup_type_name_wf: Heq => ->.
-    - move=> [flds Hlook].
-        by rewrite is_interface_type_equation_1 Hlook.
-  Qed.
- 
-
-  Lemma is_union_type_wfP (schema : wfSchema) ty :
-    reflect (exists mbs, lookup_type schema ty = Some (UnionTypeDefinition ty mbs))
-            (is_union_type schema ty).
-  Proof.
-    apply: (iffP idP).
-    - funelim (is_union_type schema ty) => // _.
-        by exists f0; rewrite Heq; move/lookup_type_name_wf: Heq => ->.
-    - move=> [mbs Hlook].
-        by rewrite is_union_type_equation_1 Hlook.
-  Qed.
-
-
-  
-  Lemma declares_implementation_are_interfaces (schema : wfSchema) tdef (ity : Name) :
-    declares_implementation schema tdef ity ->
-    is_interface_type schema ity.
-  Proof.
-    move=> Hdecl.
-    move: (declares_implementation_is_object Hdecl).
-    move/is_object_type_wfP=> [intfs [flds /lookup_in_schemaP Hlook]].
-    move: Hdecl Hlook; wfschema => Hdecl Hlook.
-    move: (Hok (tdef, ObjectTypeDefinition tdef intfs flds) Hlook).
-    rewrite is_type_def_wf_objE => /and5P [_ _ _ /allP Hintf _].
-    rewrite /declares_implementation in Hdecl.
-    move/lookup_in_schemaP: Hlook => Hlook.
-    rewrite Hlook in Hdecl.
-    by apply: (Hintf ity Hdecl).
-  Qed.    
-    
-
-  Lemma in_seq_nilN {A : eqType} (a : A) (s : seq A) :
-    a \in s -> s != [::].
-  Proof. by case: s. Qed.
-  
-  Lemma in_fset_N_fset0 {A : ordType} (a : A) (s : seq A) :
-    a \in fset s -> fset s != fset0.
-  Proof.
-      by move=> Hin; apply/fset0Pn; exists a. Qed.
-
-  
-  Lemma has_implementation_is_interface (schema : wfSchema) ty t :
-    t \in implementation schema ty ->
-    is_interface_type schema ty.
-  Proof.
-    
-    (* move/in_fset_N_fset0. *)
-    (* move/implementationP=> [tdef /codommP [t'  Hlook]]. *)
-    (* move: (lookup_type_name_wf Hlook) => Heq; rewrite Heq in Hlook. *)
-    (* move/lookup_in_schemaP: Hlook => Hin. *)
-    (* move/(implements_declares_implementation ty Hin). *)
-    (* by apply: declares_implementation_are_interfaces. *)
-  (* Qed. *)
-  Admitted.
- 
-    
-  Lemma field_in_interface_in_object (schema : wfSchema) ty ti f :
-    ty \in implementation schema ti ->
-    lookup_field_in_type schema ti f -> lookup_field_in_type schema ty f.
-  Proof.
-    move=> Hin.
-    move/declares_in_implementation: Hin => Hdecl.
-    move: (declares_implementation_is_object Hdecl) => /is_object_type_wfP.
-    case=> [intfs [flds Hlook]].
-    rewrite {2}/lookup_field_in_type Hlook.
-    move/lookup_field_in_typeP=> [tdef [ty' [Hlook' Hfin]]] Heq /=.
-    move: (lookup_type_name_wf Hlook') => Heq'.
-    rewrite /declares_implementation Hlook in Hdecl.
-    move: (lookup_type_name_wf Hlook) => Hneq.
-
-    move/lookup_in_schemaP: Hlook => Hin.
-    move: Hlook' Hin; wfschema => Hlook' Hin.
-    move: (Hok (ty, (ObjectTypeDefinition ty intfs flds)) Hin) => {Hok}.
-    rewrite is_type_def_wf_objE => /and5P [_ _ _ _ /allP Hintfs].
-    move: (Hintfs ti Hdecl) => {Hintfs Hdecl}.
-    move/implements_interface_correctlyP => H'.
-    move/lookup_in_schemaP: Hlook'.
-    rewrite Heq' => Hin'.
-    move: Hfin.
-    rewrite -(fields_E Hin') => Hfields.
-    rewrite -Heq' in Hfields.
-    move: (H' ty' Hfields) => [fld [Hfin Hok]].
-    apply/get_firstP.
-    exists fld.
-    rewrite Hneq in Hin.
-      by rewrite (fields_E Hin) in Hfin => /=.
-      apply/has_field_nameP.
-      move: Hok; rewrite /is_field_ok => [/and3P [/eqP HE]] _ _.
-      by rewrite -Heq.
-  Qed.
-
- 
-    
-        
-   Lemma field_in_interface_in_object_E (schema : wfSchema) ty ti f fld fld' :
-    ty \in implementation schema ti ->
-           lookup_field_in_type schema ti f = Some fld ->
-           [/\ lookup_field_in_type schema ty f = Some fld',
-            fld.(fname) = fld'.(fname) &
-            fld.(return_type) = fld'.(return_type)].
-  Proof.
-  Admitted.
-
-  
-  Lemma field_in_interface_in_object_same_return_type (schema : wfSchema) ty ti f fld :
-    ty \in implementation schema ti ->
-           lookup_field_in_type schema ti f = Some fld ->
-           exists2 fld', lookup_field_in_type schema ty f = Some fld' & fld.(return_type) = fld'.(return_type).
-  Admitted.
-           
-  
-  Lemma union_members_has_objects (schema : wfSchema) ty :
-    all (is_object_type schema) (union_members schema ty).
-  Proof.
-    rewrite /union_members.
-    case Hlook: lookup_type => [tdef|] //.
-    case: tdef Hlook => // u mbs /lookup_in_schemaP Hlook.
-    move: Hlook; wfschema => Hlook.
-    move/Hok: Hlook => /=.
-    by rewrite is_type_def_wf_unionE => /andP [_ Hobj].
-  Qed.
-  
-  Lemma union_members_nfset0Pwf (schema : wfSchema) ty :
-    reflect (is_union_type schema ty) (union_members schema ty != fset0).
-  Proof.
-    apply: (iffP idP).
-    - move/fset0Pn=> [x].
-      rewrite /union_members.
-      funelim (is_union_type schema ty) => //; rewrite Heq //.
-    - funelim (is_union_type schema ty) => // _.
-      rewrite /union_members Heq.
-      move/lookup_in_schemaP: Heq.
-      wfschema.
-      move/(Hok (ty, UnionTypeDefinition s2 f0)) => /=.
-      by rewrite is_type_def_wf_unionE => /andP [H _].
-  Qed.
-
-  Lemma in_union_is_object (schema : wfSchema) ty uty :
-    ty \in union_members schema uty ->
-           is_object_type schema ty.
-  Proof.
-    move=> Hin.
-    move/allP: (union_members_has_objects schema uty).
-    by move/(_ ty Hin).
-  Qed.
-  
-  Lemma in_possible_typesPwf (schema : wfSchema) t ty :
-    is_object_type schema t ->
-    reflect
-      ([\/ t = ty,
-        t \in implementation schema ty |
-        t \in union_members schema ty])
-      (t \in get_possible_types schema ty).
-  Proof.
-    move=> Hobj.
-    apply: (iffP idP).
-    - apply_funelim (get_possible_types schema ty) => //=.
-      * by move=> ty' o i flds _;  rewrite in_fset1 => /eqP ->; constructor 1.
-      * by move=> ty' i flds /lookup_type_name_wf /= ->; constructor 2.
-      * by move=> ty' u mbs Hlook; rewrite /union_members Hlook; constructor 3.
-      
-        
-    - move=> [<- | Hintfs | Hunion]; simp get_possible_types.
-      * move/is_object_type_wfP: Hobj => [intfs [flds Hlook]].
-          by rewrite Hlook; apply/fset1P.
-      * move: (declares_in_implementation schema t ty).
-        case=> _ H.
-        move: (H Hintfs) => /declares_implementation_are_interfaces.
-        move/is_interface_type_wfP=> [flds Hlook].
-        by rewrite Hlook.
-      - move: (in_union Hunion) => /is_union_type_wfP [mbs Hlook].
-        by rewrite /union_members Hlook in Hunion *.
-  Qed. 
-
-  Lemma in_possible_types_is_object (schema : wfSchema) ty :
-    forall t,
-    t \in get_possible_types schema ty ->
-          is_object_type schema t.
-  Proof.
-    funelim (get_possible_types schema ty) => // t.
-    - rewrite in_fset1 => /eqP ->.
-      by simp is_object_type; rewrite Heq.
-    - by move/in_implementation_is_object.
-    - have <-: union_members schema ty = f0 by rewrite /union_members Heq.
-        by move/in_union_is_object.
-  Qed.
-  
-  Lemma get_possible_types_interfaceE (schema : wfSchema) ty :
-    is_interface_type schema ty ->
-    get_possible_types schema ty = implementation schema ty.
-  Proof.
-    move/is_interface_type_E=> [i [flds Hlook]].
-    simp get_possible_types; rewrite Hlook.
-    by move/lookup_type_name_wf: Hlook => ->.
-  Qed.
-
-   Lemma is_subtype_obj_eq (schema : wfSchema) ty ty' :
-     is_object_type schema ty' ->
-     is_subtype schema (NT ty) (NT ty') ->
-     ty = ty'.
-   Proof.
-     funelim (is_subtype schema (NT ty) (NT ty')) => //= Hobj.
-     case: H => ->.
-     case: H0 => ->.
-     case/or3P; first by apply/eqP.
-     
-     move/declares_implementation_are_interfaces.
-     by move: (is_object_type_interfaceN Hobj) => ->.
-     move/in_union.
-     by move: (is_object_type_unionN Hobj) => ->.
-   Qed.
-
-   
-   Lemma args_are_subset_in_implementation (schema : wfSchema) ity oty  :
-     oty \in implementation schema ity ->
-      forall fld, fld \in ity.(fields schema) ->
-      exists fld', fld' \in oty.(fields schema) ->                                     
-      [/\ fld'.(fname) = fld.(fname),                
-       fsubset fld.(fargs) fld'.(fargs) &
-       is_subtype schema fld'.(return_type) fld.(return_type)].
-   Proof.
-   Admitted.
-
 
 
 End WellFormedness.
