src/theory/SchemaWFLemmas.v
@@ -1,0 +1,331 @@
+From mathcomp Require Import all_ssreflect.
+Unset Strict Implicit.
+Unset Printing Implicit Defensive.
+From extructures Require Import ord fset fmap.
+
+From Equations Require Import Equations.
+
+Require Import Schema.
+Require Import SchemaAux.
+Require Import SchemaAuxLemmas.
+Require Import SchemaWellFormedness.
+
+Section Theory.
+
+  Variable (Name Vals : ordType).
+  Variable (s : @wfSchema Name Vals).
+  
+
+
+  
+  Lemma implements_interface_correctlyP (ity ty : NamedType) :
+    reflect (forall fi, fi \in fields s ity ->
+                          exists f, f \in fields s ty /\ is_field_ok s f fi)
+            (implements_interface_correctly s ty ity).
+  Proof.
+    apply: (iffP idP).
+    - rewrite /implements_interface_correctly => /allP H.
+      by move=> fi /H /hasP [f Hin Hok]; exists f.
+    - move=> H.
+      rewrite /implements_interface_correctly.
+      apply/allP => fi Hin.
+      apply/hasP.
+      by move: (H fi Hin) => [f [Hin' Hok]]; exists f.
+  Qed.
+
+  
+  Lemma is_type_def_wf_objE name interfaces fields :
+    is_type_def_wf s (ObjectTypeDefinition name interfaces fields) =
+    [&& (fields != [::]),
+       uniq [seq fld.(fname) | fld <- fields],
+       all (is_field_wf s) fields,
+       all (is_interface_type s) interfaces &
+       all (implements_interface_correctly s name) interfaces].
+  Proof.
+      by case: sch. Qed.
+
+  Lemma is_type_def_wf_unionE name mbs :
+    is_type_def_wf s (UnionTypeDefinition name mbs) = (mbs != fset0) && all (is_object_type s) mbs.
+  Proof. by case: sch. Qed.
+
+  Ltac wfschema := case: s => sch Hhty; rewrite /is_schema_wf => /= /and4P [Hqin Hqobj Hhn /allP Hok].
+
+  Lemma query_has_object_type :
+    is_object_type s s.(query_type).
+  Proof.
+      by  wfschema.
+  Qed.
+
+
+  Lemma tdefs_N_nil :
+    s.(type_definitions) != emptym.
+  Proof.
+    wfschema.
+    rewrite /schema_names in_fset in Hqin.
+    move/mapP: Hqin => [x /codommP [t Hs] Hqin].
+    case: (type_definitions sch) Hs.
+    by case.
+  Qed.
+
+  Lemma lookup_type_name_wf ty tdef :
+    lookup_type s ty = Some tdef ->
+    ty = tdef.(tdname).
+  Proof.
+    wfschema.
+    rewrite /lookup_type.
+    move/getmP=> Hin.
+    move/allP: Hhn.
+    by move/(_ (ty, tdef) Hin) => /has_nameP /=.
+  Qed.
+
+  
+  Lemma lookup_in_schema_wfP ty tdef :
+    reflect (lookup_type s ty = Some tdef /\ ty = tdef.(tdname))
+            ((ty, tdef) \in s.(type_definitions)).
+  Proof.
+    wfschema.
+    apply: (iffP idP).
+    - move=> Hin.
+      move/allP: Hhn.
+      move/(_ (ty, tdef) Hin) => /has_nameP /= Heq.
+      rewrite Heq in Hin *.
+        by move/lookup_in_schemaP: Hin; split.
+    - move=> [Hlook Heq].
+      by apply/lookup_in_schemaP.
+  Qed.
+
+ 
+  Lemma is_scalar_type_wfE ty :
+    reflect (lookup_type s ty = Some (ScalarTypeDefinition ty))
+            (is_scalar_type s ty).
+  Proof.
+    apply: (iffP idP).
+    - rewrite /is_scalar_type.
+      case Hlook: lookup_type => [tdef|] //.
+      move/lookup_type_name_wf: Hlook => ->.
+        by case: tdef.
+    - move=> Hlook.
+      by rewrite /is_scalar_type Hlook.
+  Qed.
+
+  
+  Lemma is_object_type_wfP ty :
+    reflect (exists intfs flds, lookup_type s ty = Some (ObjectTypeDefinition ty intfs flds))
+            (is_object_type s ty).
+  Proof.
+    apply: (iffP idP)=> //.
+    - funelim (is_object_type s ty) => // _.
+      by exists interfaces, fields; rewrite Heq; move/lookup_type_name_wf: Heq => ->.
+    - move=> [intfs [flds Hlook]].
+        by rewrite is_object_type_equation_1 Hlook.
+  Qed.
+
+  Lemma is_interface_type_wfP ty :
+    reflect (exists flds, lookup_type s ty = Some (InterfaceTypeDefinition ty flds))
+            (is_interface_type s ty).
+  Proof.
+    apply: (iffP idP).
+    - funelim (is_interface_type s ty) => // _.
+        by exists fields0; rewrite Heq; move/lookup_type_name_wf: Heq => ->.
+    - move=> [flds Hlook].
+        by rewrite is_interface_type_equation_1 Hlook.
+  Qed.
+ 
+
+  Lemma is_union_type_wfP ty :
+    reflect (exists mbs, lookup_type s ty = Some (UnionTypeDefinition ty mbs))
+            (is_union_type s ty).
+  Proof.
+    apply: (iffP idP).
+    - funelim (is_union_type s ty) => // _.
+        by exists union_members; rewrite Heq; move/lookup_type_name_wf: Heq => ->.
+    - move=> [mbs Hlook].
+        by rewrite is_union_type_equation_1 Hlook.
+  Qed.
+
+    
+  Lemma declares_implementation_are_interfaces tdef (ity : Name) :
+    declares_implementation s tdef ity ->
+    is_interface_type s ity.
+  Proof.
+    move=> Hdecl.
+    move: (declares_implementation_is_object Name s ity tdef Hdecl).
+    move/is_object_type_wfP=> [intfs [flds /lookup_in_schemaP Hlook]].
+    move: Hdecl Hlook; wfschema => Hdecl Hlook.
+    move: (Hok (tdef, ObjectTypeDefinition tdef intfs flds) Hlook).
+    move=> /= /and5P [_ _ _ /allP Hintf _].
+    rewrite /declares_implementation in Hdecl.
+    move/lookup_in_schemaP: Hlook => Hlook.
+    rewrite Hlook in Hdecl.
+    by apply: (Hintf ity Hdecl).
+  Qed.
+  
+  
+  Lemma has_implementation_is_interface ty t :
+    t \in implementation s ty ->
+    is_interface_type s ty.
+  Proof.  
+  Admitted.
+
+      
+  Lemma field_in_interface_in_object ty ti f :
+    ty \in implementation s ti ->
+    lookup_field_in_type s ti f -> lookup_field_in_type s ty f.
+  Proof.
+    move=> Hin.
+    move/declares_in_implementation: Hin => Hdecl.
+    move: (declares_implementation_is_object Name s ti ty  Hdecl) => /is_object_type_wfP.
+    case=> [intfs [flds Hlook]].
+    rewrite {2}/lookup_field_in_type Hlook.
+    move/lookup_field_in_typeP=> [tdef [ty' [Hlook' Hfin]]] Heq /=.
+    move: (lookup_type_name_wf ti tdef Hlook') => Heq'.
+    rewrite /declares_implementation Hlook in Hdecl.
+    move: (lookup_type_name_wf ty _ Hlook) => Hneq.
+
+    move/lookup_in_schemaP: Hlook => Hin.
+    move: Hlook' Hin; wfschema => Hlook' Hin.
+    move: (Hok (ty, (ObjectTypeDefinition ty intfs flds)) Hin) => {Hok}.
+    move=> /= /and5P [_ _ _ _ /allP Hintfs].
+    move: (Hintfs ti Hdecl) => {Hintfs Hdecl}.
+    (* I think the problem is that it is defined on "s" which is the variable... *)
+    (* Should probably be solved by modularizing. *)
+    (* move=> /(implements_interface_correctlyP ti ty) H'. *)
+    (*   move/lookup_in_schemaP: Hlook'. *)
+    (*   rewrite Heq' => Hin'. *)
+    (*   move: Hfin. *)
+    (*   rewrite -(fields_E Hin') => Hfields. *)
+    (*   rewrite -Heq' in Hfields. *)
+    (*   move: (H' ty' Hfields) => [fld [Hfin Hok]]. *)
+    (*   apply/get_firstP. *)
+    (*   exists fld. *)
+    (*   rewrite Hneq in Hin. *)
+    (*     by rewrite (fields_E Hin) in Hfin => /=. *)
+    (*     apply/has_field_nameP. *)
+    (*     move: Hok; rewrite /is_field_ok => [/and3P [/eqP HE]] _ _. *)
+    (*     by rewrite -Heq. *)
+    (* Qed. *)
+  Admitted.
+  
+
+  
+   Lemma field_in_interface_in_object_E ty ti f fld fld' :
+    ty \in implementation s ti ->
+           lookup_field_in_type s ti f = Some fld ->
+           [/\ lookup_field_in_type s ty f = Some fld',
+            fld.(fname) = fld'.(fname) &
+            fld.(return_type) = fld'.(return_type)].
+  Proof.
+  Admitted.
+
+  
+  Lemma field_in_interface_in_object_same_return_type ty ti f fld :
+    ty \in implementation s ti ->
+           lookup_field_in_type s ti f = Some fld ->
+           exists2 fld', lookup_field_in_type s ty f = Some fld' & fld.(return_type) = fld'.(return_type).
+  Admitted.
+           
+  
+  Lemma union_members_has_objects ty :
+    all (is_object_type s) (union_members s ty).
+  Proof.
+    rewrite /union_members.
+    case Hlook: lookup_type => [tdef|] //.
+    case: tdef Hlook => // u mbs /lookup_in_schemaP Hlook.
+    move: Hlook; wfschema => Hlook.
+    move/Hok: Hlook => /=; by case/andP.
+  Qed.
+
+
+    
+
+  Lemma in_union_is_object ty uty :
+    ty \in union_members s uty ->
+           is_object_type s ty.
+  Proof.
+    move=> Hin.
+    move/allP: (union_members_has_objects uty).
+    by move/(_ ty Hin).
+  Qed.
+
+   Lemma in_possible_typesPwf t ty :
+    is_object_type s t ->
+    reflect
+      ([\/ t = ty,
+        t \in implementation s ty |
+        t \in union_members s ty])
+      (t \in get_possible_types s ty).
+  Proof.
+    move=> Hobj.
+    apply: (iffP idP).
+    - apply_funelim (get_possible_types s ty) => //=.
+      * by move=> ty' o i flds _;  rewrite in_fset1 => /eqP ->; constructor 1.
+      * by move=> ty' i flds /lookup_type_name_wf /= ->; constructor 2.
+      * by move=> ty' u mbs Hlook; rewrite /union_members Hlook; constructor 3.
+      
+        
+    - move=> [<- | Hintfs | Hunion]; simp get_possible_types.
+      * move/is_object_type_wfP: Hobj => [intfs [flds Hlook]].
+          by rewrite Hlook; apply/fset1P.
+      * move: (declares_in_implementation Name s t ty).
+        case=> _ H.
+        move: (H Hintfs) => /declares_implementation_are_interfaces.
+        move/is_interface_type_wfP=> [flds Hlook].
+        by rewrite Hlook.
+      - move: (in_union Name s t ty Hunion) => /is_union_type_wfP [mbs Hlook].
+        by rewrite /union_members Hlook in Hunion *.
+  Qed. 
+
+
+    Lemma in_possible_types_is_object ty :
+    forall t,
+    t \in get_possible_types s ty ->
+          is_object_type s t.
+  Proof.
+    funelim (get_possible_types s ty) => // t.
+    - rewrite in_fset1 => /eqP ->.
+      by simp is_object_type; rewrite Heq.
+    - by move/in_implementation_is_object.
+    - have <-: union_members s ty = union_members0 by rewrite /union_members Heq.
+        by move/in_union_is_object.
+  Qed.
+  
+  Lemma get_possible_types_interfaceE ty :
+    is_interface_type s ty ->
+    get_possible_types s ty = implementation s ty.
+  Proof.
+    move/is_interface_type_E=> [i [flds Hlook]].
+    simp get_possible_types; rewrite Hlook.
+    by move/lookup_type_name_wf: Hlook => ->.
+  Qed.
+
+   Lemma is_subtype_obj_eq ty ty' :
+     is_object_type s ty' ->
+     is_subtype s (NT ty) (NT ty') ->
+     ty = ty'.
+   Proof.
+     funelim (is_subtype s (NT ty) (NT ty')) => //= Hobj.
+     case: H => ->.
+     case: H0 => ->.
+     case/or3P; first by apply/eqP.
+     
+     move/declares_implementation_are_interfaces.
+     by move: (is_object_type_interfaceN Name s ty' Hobj) => ->.
+     move/in_union.
+     by move: (is_object_type_unionN Name s ty' Hobj) => ->.
+   Qed.
+
+   
+   Lemma args_are_subset_in_implementation ity oty  :
+     oty \in implementation s ity ->
+      forall fld, fld \in ity.(fields s) ->
+      exists fld', fld' \in oty.(fields s) ->                                     
+      [/\ fld'.(fname) = fld.(fname),                
+       fsubset fld.(fargs) fld'.(fargs) &
+       is_subtype s fld'.(return_type) fld.(return_type)].
+   Proof.
+   Admitted.
+
+
+End Theory.
+
+   
